src/SlabsCommon.fsti
@@ -121,21 +121,21 @@ let p_empty (size_class: sc) : blob -> vprop
   fun (b:blob) ->
     slab_vprop size_class (snd b) (fst b)
     `VR2.vrefine`
-    (fun ((|s,_|), _) -> is_empty size_class s == true)
+    (fun (|s,_|) -> is_empty size_class s == true)
 
 let p_partial (size_class: sc) : blob -> vprop
   =
   fun (b:blob) ->
     slab_vprop size_class (snd b) (fst b)
     `VR2.vrefine`
-    (fun ((|s,_|), _) -> is_partial size_class s == true)
+    (fun (|s,_|) -> is_partial size_class s == true)
 
 let p_full (size_class: sc) : blob -> vprop
   =
   fun (b:blob) ->
     slab_vprop size_class (snd b) (fst b)
     `VR2.vrefine`
-    (fun ((|s,_|), _) -> is_full size_class s == true)
+    (fun (|s,_|) -> is_full size_class s == true)
 
 let p_guard (size_class) : blob -> vprop
   =
@@ -155,7 +155,7 @@ val p_empty_unpack (#opened:_)
     let blob1
       : t_of (slab_vprop sc (snd b2) (fst b2))
       = h1 (slab_vprop sc (snd b2) (fst b2)) in
-    let v1 : Seq.lseq U64.t 4 = dfst (fst blob1) in
+    let v1 : Seq.lseq U64.t 4 = dfst blob1 in
     b1 == b2 /\
     is_empty sc v1 /\
     h0 ((p_empty sc) b1)
@@ -175,7 +175,7 @@ val p_partial_unpack (#opened:_)
     let blob1
       : t_of (slab_vprop sc (snd b2) (fst b2))
       = h1 (slab_vprop sc (snd b2) (fst b2)) in
-    let v1 : Seq.lseq U64.t 4 = dfst (fst blob1) in
+    let v1 : Seq.lseq U64.t 4 = dfst blob1 in
     b1 == b2 /\
     is_partial sc v1 /\
     h0 ((p_partial sc) b1)
@@ -195,7 +195,7 @@ val p_full_unpack (#opened:_)
     let blob1
       : t_of (slab_vprop sc (snd b2) (fst b2))
       = h1 (slab_vprop sc (snd b2) (fst b2)) in
-    let v1 : Seq.lseq U64.t 4 = dfst (fst blob1) in
+    let v1 : Seq.lseq U64.t 4 = dfst blob1 in
     b1 == b2 /\
     is_full sc v1 /\
     h0 ((p_full sc) b1)
@@ -232,7 +232,7 @@ val p_empty_pack (#opened:_)
     let blob0
       : t_of (slab_vprop sc (snd b1) (fst b1))
       = h0 (slab_vprop sc (snd b1) (fst b1)) in
-    let v0 : Seq.lseq U64.t 4 = dfst (fst blob0) in
+    let v0 : Seq.lseq U64.t 4 = dfst blob0 in
     is_empty sc v0 /\
     b1 == b2
   )
@@ -254,7 +254,7 @@ val p_partial_pack (#opened:_)
     let blob0
       : t_of (slab_vprop sc (snd b1) (fst b1))
       = h0 (slab_vprop sc (snd b1) (fst b1)) in
-    let v0 : Seq.lseq U64.t 4 = dfst (fst blob0) in
+    let v0 : Seq.lseq U64.t 4 = dfst blob0 in
     is_partial sc v0 /\
     b1 == b2
   )
@@ -276,7 +276,7 @@ val p_full_pack (#opened:_)
     let blob0
       : t_of (slab_vprop sc (snd b1) (fst b1))
       = h0 (slab_vprop sc (snd b1) (fst b1)) in
-    let v0 : Seq.lseq U64.t 4 = dfst (fst blob0) in
+    let v0 : Seq.lseq U64.t 4 = dfst blob0 in
     is_full sc v0 /\
     b1 == b2
   )
@@ -546,11 +546,10 @@ let size_class_vprop_aux
   : vprop
   =
   left_vprop size_class
-    (A.split_r slab_region 0sz) md_bm_region md_region
+    slab_region md_bm_region md_region
     empty_slabs partial_slabs full_slabs guard_slabs v `star`
   right_vprop
-    (A.split_r slab_region 0sz) md_bm_region md_region v `star`
-  A.varrayp (A.split_l slab_region 0sz) halfp
+    slab_region md_bm_region md_region v
 
 open SteelVRefineDep
 
@@ -656,7 +655,7 @@ val pack_slab_starseq
     = h0 (slab_vprop size_class
       (slab_array slab_region idx)
       (md_bm_array md_bm_region idx)) in
-    let md : Seq.lseq U64.t 4 = dfst (fst md_blob) in
+    let md : Seq.lseq U64.t 4 = dfst md_blob in
     //(v == 3ul ==> is_guard size_class md) /\
     (v == 3ul ==> is_guard size_class
       (slab_array slab_region idx)
@@ -682,10 +681,9 @@ val pack_right_and_refactor_vrefine_dep
     vrefinedep
       (vptr md_count)
       vrefinedep_prop
-      (left_vprop size_class (A.split_r slab_region 0sz) md_bm_region md_region r1 r2 r3 r4)
+      (left_vprop size_class slab_region md_bm_region md_region r1 r2 r3 r4)
     `star`
-    (right_vprop (A.split_r slab_region 0sz) md_bm_region md_region md_count_v `star`
-    A.varrayp (A.split_l slab_region 0sz) halfp)
+    right_vprop slab_region md_bm_region md_region md_count_v
   )
   (fun _ ->
     vrefinedep
@@ -698,7 +696,7 @@ val pack_right_and_refactor_vrefine_dep
       = h0 (vrefinedep
       (vptr md_count)
       vrefinedep_prop
-      (left_vprop size_class (A.split_r slab_region 0sz) md_bm_region md_region r1 r2 r3 r4)
+      (left_vprop size_class slab_region md_bm_region md_region r1 r2 r3 r4)
     ) in
     md_count_v == dfst blob0)
   (ensures fun h0 _ h1 ->
@@ -706,7 +704,7 @@ val pack_right_and_refactor_vrefine_dep
       = h0 (vrefinedep
       (vptr md_count)
       vrefinedep_prop
-      (left_vprop size_class (A.split_r slab_region 0sz) md_bm_region md_region r1 r2 r3 r4)
+      (left_vprop size_class slab_region md_bm_region md_region r1 r2 r3 r4)
     ) in
     let blob1
       = h1 (vrefinedep
